Changed CallS to use a new MappedCall type

theories/Ref/SpecM.v
@@ -616,6 +616,27 @@ Definition stackIncl (stk1 stk2 : FunStack) : Type :=
     forall n, n < plength stk1 ->
               nthLRT stk1 n = nthLRT stk2 (f n) /\ f n < plength stk2 }.
 
+(* Apply a stackIncl, mapping anything outside of the domain to outside of the
+codomain *)
+Definition applyIncl {stk1 stk2} (incl : stackIncl stk1 stk2) n :=
+  match Compare_dec.lt_dec n (plength stk1) with
+  | left _ => proj1_sig incl n
+  | right _ => plength stk2
+  end.
+
+(* applyIncl preserves nthLRT *)
+Lemma applyInclEq {stk1 stk2} incl n :
+  nthLRT stk2 (@applyIncl stk1 stk2 incl n) = nthLRT stk1 n.
+Proof.
+  unfold applyIncl. destruct (Compare_dec.lt_dec n (plength stk1)).
+  - symmetry. apply (proj2_sig incl n). assumption.
+  - unfold nthLRT. repeat rewrite nth_default'_default.
+    + reflexivity.
+    + destruct (Compare_dec.le_lt_dec (plength stk1) n); [ assumption | ].
+      elimtype False; apply n0; assumption.
+    + reflexivity.
+Qed.
+
 (* The trivial stack inclusion from the empty stack *)
 Program Definition nilStackIncl stk : stackIncl pnil stk :=
   fun n => n.
@@ -742,20 +763,76 @@ Proof.
     [ destruct (projT1 args) | assumption ].
 Qed.
 
-Program Definition castLRTInput stk lrt lrt' (e : lrt = lrt')
-  (args : LRTInput stk lrt) :
-  { args': LRTInput stk lrt' | LRTOutput _ _ args' = LRTOutput _ _ args } := args.
+Definition castLRTInput stk lrt lrt' (e : lrt = lrt')
+  (args : LRTInput stk lrt) : LRTInput stk lrt' :=
+  eq_rect lrt (LRTInput stk) args lrt' e.
 
-Definition StackCallWithRet stk R :=
-  { call : StackCall stk | StackCallRet stk call = R }.
+Program Definition uncastLRTOutput stk lrt lrt' (e : lrt = lrt')
+  (args : LRTInput stk lrt)
+  (ret : LRTOutput stk lrt' (castLRTInput _ lrt lrt' e args)) :
+  LRTOutput stk lrt args := _.
 
-Definition StackCallS E stk (args : StackCall stk)
-  : SpecM E stk (StackCallRet stk args) :=
-  trigger (H2:=@SpecEventReSumRet _ _ _ _ _ _) args.
+(* A StackCall to a function in stk1 with args relative to stk2; the idea is
+that it is being "mapped" from stk1 to stk2 *)
+Inductive MappedCall stk1 stk2 : Type@{entree_u} :=
+| MappedCallOfArgs n (args : LRTInput stk2 (nthLRT stk1 n)).
 
-Definition CallS E stk R (call : StackCallWithRet stk R) : SpecM E stk R :=
-  bind (StackCallS E stk (proj1_sig call))
-    (fun r => ret (eq_rect _ (fun T => T) r R (proj2_sig call))).
+(* The return type for a MappedCall recursive call *)
+Definition MappedCallRet stk1 stk2 (call: MappedCall stk1 stk2) : Type@{entree_u} :=
+  match call with
+  | MappedCallOfArgs _ _ n args => LRTOutput stk2 (nthLRT stk1 n) args
+  end.
+
+(* Convert a MappedCall to the StackCall it is meant to be mapped to *)
+Definition mapMappedCall stk1 stk2 (incl : stackIncl stk1 stk2)
+  (call : MappedCall stk1 stk2) : StackCall stk2 :=
+  match call with
+  | MappedCallOfArgs _ _ n args =>
+      StackCallOfArgs stk2 (applyIncl incl n)
+        (castLRTInput stk2 _ _ (eq_sym (applyInclEq incl n)) args)
+  end.
+
+(* Convert a StackCallRet back to a MappedCallRet *)
+Definition unmapMappedCallRet stk1 stk2 (incl : stackIncl stk1 stk2)
+  (call : MappedCall stk1 stk2) :
+  StackCallRet _ (mapMappedCall _ _ incl call) ->
+  MappedCallRet stk1 stk2 call :=
+  match call return StackCallRet _ (mapMappedCall _ _ incl call) ->
+                    MappedCallRet stk1 stk2 call with
+  | MappedCallOfArgs _ _ n args =>
+      uncastLRTOutput _ _ _ (eq_sym (applyInclEq incl n)) args
+  end.
+
+(* Tell the typeclass system to look for stackIncl assumptions *)
+Global Hint Extern 1 (stackIncl _ _) => assumption : typeclass_instances.
+
+Global Instance EncodingType_MappedCall stk1 stk2
+  : EncodingType (MappedCall stk1 stk2) := MappedCallRet stk1 stk2.
+
+Global Program Instance ReSum_MappedCall stk1 stk2 (incl : stackIncl stk1 stk2) :
+  ReSum (MappedCall stk1 stk2) (StackCall stk2) :=
+  mapMappedCall stk1 stk2 incl.
+
+Global Program Instance ReSumRet_MappedCall stk1 stk2
+  (incl : stackIncl stk1 stk2) :
+  ReSumRet (MappedCall stk1 stk2) (StackCall stk2) :=
+  unmapMappedCallRet stk1 stk2 incl.
+
+Global Program Instance ReSum_MappedCall_FunStackE E stk1 stk2
+  (incl : stackIncl stk1 stk2) :
+  ReSum (MappedCall stk1 stk2) (FunStackE E stk2) :=
+  fun args => inl (mapMappedCall _ _ incl args).
+
+Global Program Instance ReSumRet_MappedCall_FunStackE E stk1 stk2
+  (incl : stackIncl stk1 stk2) :
+  ReSumRet (MappedCall stk1 stk2) (FunStackE E stk2) :=
+  fun args ret => unmapMappedCallRet _ _ incl args ret.
+
+Definition CallS E stk1 stk2 (incl : stackIncl stk1 stk2)
+  (call : MappedCall stk1 stk2) : SpecM E stk2 (encodes call) :=
+  trigger call.
+
+FIXME HERE NOW
 
 Definition mkStackCall stk stk' (incl : stackIncl stk stk') n
   : lrtPi stk' (nthLRT stk n)
